Updates to the heap model

examples/seplogic/SepLogic.Heap.fsti
@@ -4,171 +4,190 @@ module S  = FStar.Set
 module TS = FStar.TSet
 
 let set  = Set.set
-let tset = TSet.set
+
+(* heaps, memories, and operations on them *)
 
 val heap : Type u#1
-val memory : Type u#1
-
-val defined : memory -> Type0
+val raw_memory : Type u#1
+val defined : raw_memory -> Type0
+let memory = m:raw_memory{defined m}
 
 val emp : memory
 
-val emp_defined : unit -> Lemma (defined emp)
+val lemma_defined_emp (u:unit) 
+  : Lemma (defined emp)
+
+assume Emp_defined_axiom : defined emp
 
 val ref (a:Type0) : Type0
 val addr_of : #a:Type0 -> ref a -> GTot nat
-
 val heap_memory : heap -> GTot memory
 
-val heap_memory_defined (h:heap)
-  : Lemma (defined (heap_memory h))
-          [SMTPat (defined (heap_memory h))]
-
-let hpred = heap -> Type0
-let mpred = memory -> Type0
-
 val disjoint_heaps : heap -> heap -> Type0
-val disjoint_memories : memory -> memory -> Type0
+val disjoint_memories : raw_memory -> raw_memory -> Type0
 
-val disjoint_heaps_comm (h0 h1:heap)
+val join : h0:heap -> h1:heap{disjoint_heaps h0 h1} -> Tot heap
+
+val ( |> ) : #a:Type0 -> r:ref a -> x:a -> GTot memory
+val ( <*> ) : m0:raw_memory -> m1:raw_memory -> GTot raw_memory
+
+val split_heap : (m0:raw_memory) 
+              -> (m1:raw_memory)
+              -> (h:heap{defined (m0 <*> m1) /\ heap_memory h == (m0 <*> m1)}) 
+              -> heap * heap
+
+val hcontains : #a:Type0 -> heap -> ref a -> Type0
+val mcontains : #a:Type0 -> raw_memory -> ref a -> Type0
+
+val sel : #a:Type0 -> h:heap -> r:ref a{h `hcontains` r} -> Tot a
+val upd : #a:Type0 -> h:heap -> r:ref a{h `hcontains` r} -> x:a -> Tot heap
+
+val fresh : #a:Type0 -> ref a -> heap -> Type0
+val alloc : #a:Type0 -> h:heap -> a -> Tot (ref a * heap) 
+
+val addrs_in : raw_memory -> Set.set nat
+
+(* disjoint_heaps and disjoint_memories *)
+
+val lemma_disjoint_heaps_comm (h0 h1:heap)
   : Lemma (disjoint_heaps h0 h1 <==> disjoint_heaps h1 h0)
 
-val disjoint_memories_emp (m:memory)
+val lemma_disjoint_memories_emp (m:raw_memory)
   : Lemma (requires (defined m))
           (ensures  (disjoint_memories m emp))
           [SMTPat (disjoint_memories m emp)]
 
-val disjoint_memories_comm (m0 m1:memory)
+val lemma_disjoint_memories_comm (m0 m1:raw_memory)
   : Lemma (requires (defined m0 /\ defined m1))
           (ensures  (disjoint_memories m0 m1 <==> disjoint_memories m1 m0))
 
-val disjoint_heaps_memories (h0 h1:heap)
+val lemma_disjoint_heaps_memories (h0 h1:heap)
   : Lemma (disjoint_heaps h0 h1 <==> disjoint_memories (heap_memory h0) (heap_memory h1))
           [SMTPat (disjoint_memories (heap_memory h0) (heap_memory h1))]
 
-val join : h0:heap -> h1:heap{disjoint_heaps h0 h1} -> Tot heap
+val lemma_sep_disjoint_memories (m0 m1:raw_memory) 
+  : Lemma (disjoint_memories m0 m1 <==> defined (m0 <*> m1))
+          [SMTPat (disjoint_memories m0 m1);
+           SMTPat (defined (m0 <*> m1))]
 
-val join_comm (h0 h1:heap)
+(* join *)
+
+val lemma_join_comm (h0 h1:heap)
   : Lemma (requires (disjoint_heaps h0 h1 /\ disjoint_heaps h1 h0))
           (ensures  (join h0 h1 == join h1 h0))
 
-val ( |> ) : #a:Type0 -> r:ref a -> x:a -> GTot memory
-val ( <*> ) : m0:memory -> m1:memory -> GTot memory
+(* <*> *)
 
-val sep_emp (m:memory)
+val lemma_sep_unit (m:raw_memory)
   : Lemma ((m <*> emp) == m)
           [SMTPat (m <*> emp)]
 
-val sep_comm (m0 m1:memory)
+val lemma_sep_comm (m0 m1:raw_memory)
   : Lemma ((m0 <*> m1) == (m1 <*> m0))
           
-val sep_assoc (m0 m1 m2:memory)
+val lemma_sep_assoc (m0 m1 m2:raw_memory)
   : Lemma ((m0 <*> (m1 <*> m2)) == ((m0 <*> m1) <*> m2))
-          [SMTPat (m0 <*> (m1 <*> m2));
-           SMTPat ((m0 <*> m1) <*> m2)]
+         [SMTPatOr [[SMTPat ((m0 <*> (m1 <*> m2)))];
+	            [SMTPat ((m0 <*> m1) <*> m2)]]]
 
-val sep_join (h0 h1:heap)
+(* heap_memory *)
+
+val lemma_sep_join (h0 h1:heap)
   : Lemma (requires (disjoint_heaps h0 h1))
           (ensures  (heap_memory (join h0 h1) == ((heap_memory h0) <*> (heap_memory h1))))
-          [SMTPat (heap_memory (join h0 h1))]          
+          [SMTPat (heap_memory (join h0 h1))]
 
-val points_to_disjoint_memories (#a:Type0) (#b:Type0) (r:ref a) (s:ref b) (x:a) (y:b)
-  : Lemma ((addr_of r <> addr_of s) <==> (disjoint_memories (r |> x) (s |> y)))
-          [SMTPat (disjoint_memories (r |> x) (s |> y))]
+(* defined *)
 
-val sep_disjoint_memories (m0 m1:memory)
-  : Lemma (disjoint_memories m0 m1 <==> defined (m0 <*> m1))
-          [SMTPat (defined (m0 <*> m1));
-           SMTPat (disjoint_memories m0 m1)]
-
-val points_to_defined (#a:Type0) (r:ref a) (x:a)
+val lemma_points_to_defined (#a:Type0) (r:ref a) (x:a)
   : Lemma (defined (r |> x))
           [SMTPat (defined (r |> x))]
 
-val sep_defined (m0 m1:memory)
+val lemma_sep_defined (m0 m1:raw_memory)
   : Lemma (requires (defined (m0 <*> m1)))
           (ensures  (defined m0 /\ defined m1))
-          [SMTPat (defined (m0 <*> m1));
-           SMTPat (defined m0);
-           SMTPat (defined m1)]
 
-val split_heap : (m0:memory) 
-              -> (m1:memory)
-              -> (h:heap{defined (m0 <*> m1) /\ heap_memory h == (m0 <*> m1)}) 
-              -> heap * heap
+(* split_heap *)
 
-val split_heap_disjoint (m0 m1:memory) (h:heap)
+val lemma_split_heap_disjoint (m0 m1:raw_memory) (h:heap)
   : Lemma (requires (defined (m0 <*> m1) /\ heap_memory h == (m0 <*> m1)))
           (ensures  (let (h0,h1) = split_heap m0 m1 h in
                      disjoint_heaps h0 h1))
           [SMTPat (split_heap m0 m1 h)]
 
-val split_heap_join (m0 m1:memory) (h:heap)
+val lemma_split_heap_join (m0 m1:raw_memory) (h:heap)
   : Lemma (requires (defined (m0 <*> m1) /\ heap_memory h == (m0 <*> m1)))
           (ensures  (let (h0,h1) = split_heap m0 m1 h in
                      h == join h0 h1))
           [SMTPat (split_heap m0 m1 h)]
 
-val split_heap_memories (m0 m1:memory) (h:heap)
+val lemma_split_heap_memories (m0 m1:raw_memory) (h:heap)
   : Lemma (requires (defined (m0 <*> m1) /\ heap_memory h == (m0 <*> m1)))
           (ensures  (let (h0,h1) = split_heap m0 m1 h in
                      heap_memory h0 == m0 /\ heap_memory h1 == m1))
           [SMTPat (split_heap m0 m1 h)]
 
-val hcontains : #a:Type0 -> heap -> ref a -> Type0
-val mcontains : #a:Type0 -> memory -> ref a -> Type0
+(* hcontains and mcontains *)
 
-val hcontains_mcontains (#a:Type0) (r:ref a) (h:heap)
+val lemma_hcontains_mcontains (#a:Type0) (r:ref a) (h:heap)
   : Lemma (h `hcontains` r <==> (heap_memory h) `mcontains` r)
           [SMTPat ((heap_memory h) `mcontains` r)]
 
-val points_to_mcontains (#a:Type0) (r:ref a) (x:a)
+val lemma_points_to_mcontains (#a:Type0) (r:ref a) (x:a)
   : Lemma ((r |> x) `mcontains` r)
           [SMTPat ((r |> x) `mcontains` r)]
 
-val sel : #a:Type0 -> h:heap -> r:ref a{h `hcontains` r} -> Tot a
-val upd : #a:Type0 -> h:heap -> r:ref a{h `hcontains` r} -> x:a -> Tot heap
+(* sel, upd, and |> *)
 
-val points_to_sel (#a:Type) (r:ref a) (x:a) (h:heap)
-  : Lemma (requires (h `hcontains` r /\ heap_memory h == (r |> x)))    //F* doesn't see that (h `hcontains` r) follows from (heap_memory h == (r |> x))
+val lemma_points_to_sel (#a:Type) (r:ref a) (x:a) (h:heap)
+  : Lemma (requires (h `hcontains` r /\ heap_memory h == (r |> x)))
           (ensures  (sel h r == x))
           [SMTPat (heap_memory h);
            SMTPat (r |> x);
            SMTPat (sel h r)]
 
-val points_to_upd (#a:Type) (r:ref a) (x:a) (v:a) (h:heap)
-  : Lemma  (requires (h `hcontains` r /\ heap_memory h == (r |> x)))  //F* doesn't see that (h `hcontains` r) follows from (heap_memory h == (r |> x))
+val lemma_points_to_upd (#a:Type) (r:ref a) (x:a) (v:a) (h:heap)
+  : Lemma  (requires (h `hcontains` r /\ heap_memory h == (r |> x)))
            (ensures  (heap_memory (upd h r v) == (r |> v)))
            [SMTPat (heap_memory h);
             SMTPat (r |> x);
             SMTPat (upd h r v)]
 
-val hfresh : #a:Type0 -> ref a -> hpred
-val mfresh : #a:Type0 -> ref a -> mpred
+(* alloc and fresh *)
 
-val hfres_mfresh (#a:Type0) (r:ref a) (h:heap)
-  : Lemma (hfresh r h <==> mfresh r (heap_memory h))
-          [SMTPat (mfresh r (heap_memory h))]
-
-val alloc : #a:Type0 -> h:heap -> a -> Tot (ref a * heap) 
-
-val alloc_fresh (#a:Type0) (h0:heap) (x:a)
+val lemma_alloc_fresh (#a:Type0) (h0:heap) (x:a)
   : Lemma (let (r,_) = alloc h0 x in
-           hfresh r h0)
+           fresh r h0)
           [SMTPat (alloc h0 x)]
 
-val alloc_contains (#a:Type0) (h0:heap) (x:a)
+val lemma_alloc_contains (#a:Type0) (h0:heap) (x:a)
   : Lemma (let (r,h1) = alloc h0 x in 
            h1 `hcontains` r)
           [SMTPat (alloc h0 x)]
 
-val alloc_sel (#a:Type0) (h0:heap) (x:a)
+val lemma_alloc_sel (#a:Type0) (h0:heap) (x:a)
   : Lemma (let (r,h1) = alloc h0 x in
            sel h1 r == x)
           [SMTPat (alloc h0 x)]
 
-val alloc_emp_points_to (#a:Type0) (h0:heap) (x:a)
+val lemma_alloc_emp_points_to (#a:Type0) (h0:heap) (x:a)
   : Lemma (requires (heap_memory h0 == emp))
           (ensures  (let (r,h1) = alloc h0 x in
                      heap_memory h1 == (r |> x)))
           [SMTPat (alloc h0 x)]
+
+(* addrs_in *)
+
+val lemma_addrs_in_emp (u:unit) 
+  : Lemma (Set.equal (addrs_in emp) (Set.empty))
+
+assume Addrs_in_emp_axiom: Set.equal (addrs_in emp) (Set.empty)
+
+val lemma_addrs_in_points_to (#a:Type) (r:ref a) (x:a)
+  : Lemma (Set.equal (addrs_in (r |> x)) (Set.singleton (addr_of r)))
+          [SMTPat (addrs_in (r |> x))]
+
+val lemma_addrs_in_join (m0 m1:raw_memory)
+  : Lemma (requires (defined (m0 <*> m1)))
+          (ensures  (Set.equal (addrs_in (m0 <*> m1)) (Set.union (addrs_in m0) (addrs_in m1))))
+          [SMTPat (addrs_in (m0 <*> m1))]
